Substitution and annotation substitution are now functions

src/Language/PlutusIR/Semantics/Dynamic/AnnotationSubstitution.v
@@ -19,144 +19,112 @@ Definition bound_tyvars_in_binding (b : NamedTerm.Binding) : list tyname :=
 
 Definition bound_tyvars_in_bindings (bs : list NamedTerm.Binding) : list tyname := List.concat (map bound_tyvars_in_binding bs).
 
-(** ** Implementation as an inductive datatype *)
-Inductive substituteA : tyname -> Ty -> Term -> Term -> Prop :=
-  | SA_Let1 : forall X S bs t0 bs',
-      In X (bound_tyvars_in_bindings bs) ->
-      substituteA_bindings_nonrec X S bs bs' ->
-      substituteA X S (Let NonRec bs t0) (Let NonRec bs' t0)
-  | SA_Let2 : forall X S bs t0 bs' t0',
-      ~(In X (bound_tyvars_in_bindings bs)) ->
-      substituteA_bindings_nonrec X S bs bs' ->
-      substituteA X S t0 t0' ->
-      substituteA X S (Let NonRec bs t0) (Let NonRec bs' t0')
-  | SA_LetRec1 : forall X S bs t0,
-      In X (bound_tyvars_in_bindings bs)->
-      substituteA X S (Let Rec bs t0) (Let Rec bs t0)
-  | SA_LetRec2 : forall X S bs t0 bs' t0',
-      ~(In X (bound_tyvars_in_bindings bs)) ->
-      substituteA_bindings_rec X S bs bs' ->
-      substituteA X S t0 t0' ->
-      substituteA X S (Let Rec bs t0) (Let Rec bs' t0')
-  | SA_Var : forall X S x,
-      substituteA X S (Var x) (Var x)
-  | SA_TyAbs1 : forall X S K t0,
-      substituteA X S (TyAbs X K t0) (TyAbs X K t0)
-  | SA_TyAbs2 : forall X S bX K t0 t0',
-      X <> bX ->
-      substituteA X S t0 t0' ->
-      substituteA X S (TyAbs bX K t0) (TyAbs bX K t0')
-  | SA_LamAbs : forall X S bx T t0 t0',
-      substituteA X S t0 t0' ->
-      substituteA X S (LamAbs bx T t0) (LamAbs bx (substituteT X S T) t0')
-  | SA_Apply : forall X S t1 t2 t1' t2',
-      substituteA X S t1 t1' ->
-      substituteA X S t2 t2' ->
-      substituteA X S (Apply t1 t2) (Apply t1' t2')
-  | SA_Constant : forall X S u,
-      substituteA X S (Constant u) (Constant u)
-  | SA_Builtin : forall X S d,
-      substituteA X S (Builtin d) (Builtin d)
-  | SA_TyInst : forall X S t0 T t0',
-      substituteA X S t0 t0' ->
-      substituteA X S (TyInst t0 T) (TyInst t0' (substituteT X S T))
-  | SA_Error : forall X S T,
-      substituteA X S (Error T) (Error (substituteT X S T))
-  | SA_IWrap : forall X S F T t0 t0',
-      substituteA X S t0 t0' ->
-      substituteA X S (IWrap F T t0) (IWrap (substituteT X S F) (substituteT X S T) t0')
-  | SA_Unwrap : forall X S t0 t0',
-      substituteA X S t0 t0' ->
-      substituteA X S (Unwrap t0) (Unwrap t0') 
-      
-with substituteA_bindings_nonrec : tyname -> Ty -> list Binding -> list Binding -> Prop :=
-  | SA_NilB_NonRec : forall X S, 
-      substituteA_bindings_nonrec X S nil nil
-  | SA_ConsB_NonRec1 : forall X S b b' bs,
-      In X (bound_tyvars_in_binding b) ->
-      substituteA_binding X S b b' ->
-      substituteA_bindings_nonrec X S (b :: bs) (b' :: bs)
-  | SA_ConsB_NonRec2 : forall X S b b' bs bs',
-      ~(In X (bound_tyvars_in_binding b)) ->
-      substituteA_binding X S b b' ->
-      substituteA_bindings_nonrec X S bs bs' ->
-      substituteA_bindings_nonrec X S (b :: bs) (b' :: bs')
+Section SubstABindings.
+  Context {substAb : tyname -> Ty -> Binding -> Binding}.
 
-with substituteA_bindings_rec : tyname -> Ty -> list Binding -> list Binding -> Prop :=
-  | SA_NilB_Rec : forall X S,
-      substituteA_bindings_rec X S nil nil
-  | SA_ConsB_Rec : forall X S b b' bs bs',
-      substituteA_binding X S b b' ->
-      substituteA_bindings_rec X S bs bs' ->
-      substituteA_bindings_rec X S (b :: bs) (b' :: bs')
+  Fixpoint substituteA_bindings_nonrec (X : tyname) (U : Ty) (bs : list Binding) : list Binding :=
+    match bs with
+    | nil => 
+        nil
+    | b :: bs' => 
+        if find (eqb X) (bound_tyvars_in_binding b)
+          then
+            substAb X U b :: bs
+          else
+            substAb X U b :: substituteA_bindings_nonrec X U bs'
+    end.
 
-with substituteA_binding : tyname -> Ty -> Binding -> Binding -> Prop :=
-  | SA_TermBind : forall X S strictness bx T t t',
-      substituteA X S t t' ->
-      substituteA_binding X S (TermBind strictness (VarDecl bx T) t) (TermBind strictness (VarDecl bx (substituteT X S T)) t')
-  | SA_TypeBind : forall X S tvd T,
-      substituteA_binding X S (TypeBind tvd T) (TypeBind tvd (substituteT X S T))
-  | SA_DatatypeBind : forall X S tvd YKs matchFunc cs cs',
-      substituteA_constructors X S cs cs' ->
-      substituteA_binding X S (DatatypeBind (Datatype tvd YKs matchFunc cs)) (DatatypeBind (Datatype tvd YKs matchFunc cs'))
-      
-with substituteA_constructors : tyname -> Ty -> list constructor -> list constructor -> Prop :=
-  | SA_NilC : forall X S,
-      substituteA_constructors X S nil nil
-  | SA_ConsC : forall X S c c' cs cs',
-      substituteA_constructor X S c c' ->
-      substituteA_constructors X S cs cs' ->
-      substituteA_constructors X S (c :: cs) (c' :: cs')
+  Fixpoint substituteA_bindings_rec (X : tyname) (U : Ty) (bs : list Binding) : list Binding :=
+    match bs with
+    | nil =>
+        nil
+    | b :: bs' =>
+        substAb X U b :: substituteA_bindings_rec X U bs'
+    end.
 
-with substituteA_constructor : tyname -> Ty -> constructor -> constructor -> Prop :=
-  | SA_Constr : forall X S T bx ar,
-      substituteA_constructor X S (Constructor (VarDecl bx T) ar) (Constructor (VarDecl bx (substituteT X S T)) ar)
-.
+End SubstABindings.
 
-#[export] Hint Constructors substituteA : core.
-#[export] Hint Constructors substituteA_bindings_nonrec : core.
-#[export] Hint Constructors substituteA_bindings_rec : core.
-#[export] Hint Constructors substituteA_binding : core.
+Section SubstAConstructors.
 
-Scheme substituteA__ind := Minimality for substituteA Sort Prop
-  with substituteA_bindings_nonrec__ind := Minimality for substituteA_bindings_nonrec Sort Prop
-  with substituteA_bindings_rec__ind := Minimality for substituteA_bindings_rec Sort Prop
-  with substituteA_binding__ind := Minimality for substituteA_binding Sort Prop.
+  Definition substituteA_constructor (X : tyname) (U : Ty) (c : constructor) : constructor :=
+    match c with
+    | Constructor (VarDecl bx T) ar =>
+        Constructor (VarDecl bx (substituteT X U T)) ar
+    end.
 
-Combined Scheme substituteA__mutind from 
-  substituteA__ind, 
-  substituteA_bindings_nonrec__ind, 
-  substituteA_bindings_rec__ind, 
-  substituteA_binding__ind.
+  Definition substituteA_constructors (X : tyname) (U : Ty) (cs : list constructor) : list constructor :=
+    map (substituteA_constructor X U) cs.
+
+End SubstAConstructors.
 
 
+Fixpoint substituteA (X : tyname) (U : Ty) (t : Term) : Term :=
+  match t with
+  | Let NonRec bs t0 =>
+      Let NonRec (@substituteA_bindings_nonrec substituteA_binding X U bs)
+        (if existsb (eqb X) (bound_tyvars_in_bindings bs) 
+          then t0
+          else substituteA X U t0
+        ) 
+  | Let Rec bs t0 =>
+      if existsb (eqb X) (bound_tyvars_in_bindings bs) 
+        then 
+          Let Rec bs t0
+        else
+          Let Rec (@substituteA_bindings_rec substituteA_binding X U bs) (substituteA X U t0)
+  | Var y => 
+      Var y
+  | TyAbs bX K t0 =>
+      if X =? bX
+        then TyAbs bX K t0
+        else TyAbs bX K (substituteA X U t0)
+  | LamAbs bx T t0 =>
+      LamAbs bx (substituteT X U T) (substituteA X U t0)
+  | Apply t1 t2 =>
+      Apply (substituteA X U t1) (substituteA X U t2)
+  | Constant u =>
+      Constant u
+  | Builtin d =>
+      Builtin d
+  | TyInst t0 T =>
+      TyInst (substituteA X U t0) (substituteT X U T)
+  | Error T =>
+      Error (substituteT X U T)
+  | IWrap F T t0 =>
+      IWrap (substituteT X U F) (substituteT X U T) (substituteA X U t0)
+  | Unwrap t0 =>
+      Unwrap (substituteA X U t0)
+  end
+
+with substituteA_binding (X : tyname) (U : Ty) (b : Binding) {struct b} : Binding :=
+  match b with
+  | TermBind stricty (VarDecl y T) tb =>
+      TermBind stricty (VarDecl y (substituteT X U T)) (substituteA X U tb)
+  | TypeBind tvd T => 
+      TypeBind tvd (substituteT X U T)
+  | DatatypeBind (Datatype tvd YKs matchFunc cs) =>
+      DatatypeBind (Datatype tvd YKs matchFunc (substituteA_constructors X U cs))
+  end.
+
+Notation "'[[' U '/' X ']' t" := (substituteA X U t) (in custom plutus_term at level 20, X constr).
+Notation "'[[' U '/' X '][b]' b" := (substituteA_binding X U b) (in custom plutus_term at level 20, X constr).
+Notation "'[[' U '/' X '][bnr]' bs" := (@substituteA_bindings_nonrec substituteA_binding X U bs) (in custom plutus_term at level 20, X constr).
+Notation "'[[' U '/' X '][br]' bs" := (@substituteA_bindings_rec substituteA_binding X U bs) (in custom plutus_term at level 20, X constr).
+Notation "'[[' U '/' X '][cs]' cs" := (substituteA_constructors X U cs) (in custom plutus_term at level 20, X constr).
+Notation "'[[' U '/' X '][c]' c" := (substituteA_constructor X U c) (in custom plutus_term at level 20, X constr).
 
 (** * Multi-substitutions of types in type annotations *)
 
 Definition envA := list (tyname * Ty).
 
-Inductive msubstA : envA -> Term -> Term -> Prop :=
-  | msubstA_nil : forall t,
-      msubstA nil t t
-  | msubstA_cons : forall a T ss t t' t'',
-      substituteA a T t t' ->
-      msubstA ss t' t'' ->
-      msubstA ((a, T) :: ss) t t''
-  .
+Fixpoint msubstA_term (ss : envA) (t : Term) : Term :=
+  match ss with
+  | nil => t
+  | (X, U) :: ss' => msubstA_term ss' <{ [[U / X] t }>
+  end.
 
-Inductive msubstA_binding : envA -> Binding -> Binding -> Prop :=
-  | msubstA_binding__nil : forall b,
-      msubstA_binding nil b b 
-  | msubstA_binding__cons : forall a T ss b b' b'',
-      substituteA_binding a T b b' ->
-      msubstA_binding ss b' b'' ->
-      msubstA_binding ((a, T) :: ss) b b''.
-
-
-Inductive msubstA_bindings_nonrec : env -> list Binding -> list Binding -> Prop :=
-| msubstA_bindings_nonrec__nil : forall bs,
-    msubstA_bindings_nonrec nil bs bs
-| msubstA_bindings_nonrec__cons : forall a T ss bs bs' bs'',
-    substituteA_bindings_nonrec a T bs bs' ->
-    msubstA_bindings_nonrec ss bs' bs'' ->
-    msubstA_bindings_nonrec ((a, T) :: ss) bs bs''.
+Fixpoint msubstA_binding (ss : envA) (b : Binding) : Binding :=
+  match ss with
+  | nil => b
+  | (X, U) :: ss' => msubstA_binding ss' <{ [[U / X][b] b }>
+  end.
