src/Language/PlutusIR/Semantics/Dynamic/AnnotationSubstitution/PreservesValue.v
@@ -7,30 +7,26 @@ Require Import PlutusCert.Language.PlutusIR.Semantics.Dynamic.AnnotationSubstitu
 
 
 
-Theorem substituteA_preserves_value : forall v v' a T,
+Theorem substituteA_preserves_value : forall v a T,
     value v ->
-    substituteA a T v v' ->
-    value v'.
+    value <{ [[T / a] v }>.
 Proof.
   intros.
   inversion H; subst; try solve [inversion H0; subst; auto]. 
 Admitted.
 
-Theorem msubstA_preserves_value : forall envA v v',
+Theorem msubstA_preserves_value : forall envA v,
     value v ->
-    msubstA envA v v' ->
-    value v'.
+    value (msubstA_term envA v).
 Proof.
   induction envA.
   - intros.
-    inversion H0.
-    subst.
+    simpl.
     assumption.
   - intros.
-    inversion H0.
-    subst.
+    simpl.
+    destruct a.
     eapply IHenvA.
-    + eapply substituteA_preserves_value; eauto.
-    + eauto.
+    eapply substituteA_preserves_value; eauto.
 Qed. 
 
