src/Language/PlutusIR/Semantics/Dynamic/Substitution.v
@@ -25,109 +25,97 @@ Definition bound_vars_in_binding (b : NamedTerm.Binding) : list string :=
 
 Definition bound_vars_in_bindings (bs : list NamedTerm.Binding) : list string := List.concat (map bound_vars_in_binding bs).
 
-(** ** Implementation of substitution on terms as inductive datatype *)
-Inductive substitute (x : name) (s : Term) :Term -> Term -> Prop :=
-  | S_LetNonRec_Nil1 : forall t t', 
-      substitute x s t t' ->
-      substitute x s (Let NonRec nil t) (Let NonRec nil t')
-  | S_LetNonRec_Cons1 : forall b b' bs t,
-      In x (bound_vars_in_binding b) ->
-      substitute_binding x s b b' ->
-      substitute x s (Let NonRec (b :: bs) t) (Let NonRec (b' :: bs) t)
-  | S_LetNonRec_Cons2 : forall b b' bs bs' t t',
-      ~(In x (bound_vars_in_binding b)) ->
-      substitute_binding x s b b' ->
-      substitute x s (Let NonRec bs t) (Let NonRec bs' t') ->
-      substitute x s (Let NonRec (b :: bs) t) (Let NonRec (b' :: bs') t')
-  | S_LetRec1 : forall bs t0,
-      In x (bound_vars_in_bindings bs)->
-      substitute x s (Let Rec bs t0) (Let Rec bs t0)
-  | S_LetRec2 : forall bs t0 bs' t0',
-      ~(In x (bound_vars_in_bindings bs)) ->
-      substitute_letrec x s (Let Rec bs t0) (Let Rec bs' t0') ->
-      substitute x s (Let Rec bs t0) (Let Rec bs' t0')
-  | S_Var1 :
-      substitute x s (Var x) s
-  | S_Var2 : forall y,
-      x <> y ->
-      substitute x s (Var y) (Var y)
-  | S_TyAbs : forall bX K t0 t0',
-      substitute x s t0 t0' ->
-      substitute x s (TyAbs bX K t0) (TyAbs bX K t0')
-  | S_LamAbs1 : forall T t0,
-      substitute x s (LamAbs x T t0) (LamAbs x T t0)
-  | S_LamAbs2 : forall bx T t0 t0',
-      x <> bx ->
-      substitute x s t0 t0' ->
-      substitute x s (LamAbs bx T t0) (LamAbs bx T t0') 
-  | S_Apply : forall t1 t2 t1' t2',
-      substitute x s t1 t1' ->
-      substitute x s t2 t2' ->
-      substitute x s (Apply t1 t2) (Apply t1' t2')
-  | S_Constant : forall u,
-      substitute x s (Constant u) (Constant u)
-  | S_Builtin : forall d,
-      substitute x s (Builtin d) (Builtin d)
-  | S_TyInst : forall t0 T t0',
-      substitute x s t0 t0' ->
-      substitute x s (TyInst t0 T) (TyInst t0' T)
-  | S_Error : forall T,
-      substitute x s (Error T) (Error T)
-  | S_IWrap : forall F T t0 t0',
-      substitute x s t0 t0' ->
-      substitute x s (IWrap F T t0) (IWrap F T t0')
-  | S_Unwrap : forall t0 t0',
-      substitute x s t0 t0' ->
-      substitute x s (Unwrap t0) (Unwrap t0') 
 
-with substitute_letrec (x : name) (s : Term) : Term -> Term -> Prop :=
-  | S_NilB_Rec : forall t t',
-      substitute x s t t' ->
-      substitute_letrec x s (Let Rec nil t) (Let Rec nil t')
-  | S_ConsB_Rec : forall b b' bs bs' t t',
-      substitute_binding x s b b' ->
-      substitute_letrec x s (Let Rec bs t) (Let Rec bs' t') ->
-      substitute_letrec x s (Let Rec (b :: bs) t) (Let Rec (b' :: bs') t')
 
-with substitute_binding (x : name) (s : Term) : Binding -> Binding -> Prop :=
-  | S_TermBind : forall strictness bx T t t',
-      substitute x s t t' ->
-      substitute_binding x s (TermBind strictness (VarDecl bx T) t) (TermBind strictness (VarDecl bx T) t')
-  | S_TypeBind : forall tvd T,
-      substitute_binding x s (TypeBind tvd T) (TypeBind tvd T)
-  | S_DatatypeBind : forall dtd,
-      substitute_binding x s (DatatypeBind dtd) (DatatypeBind dtd).
+Section SubstBindings.
+  Context {substb : name -> Term -> Binding -> Binding}.
 
-#[export] Hint Constructors substitute : core.
-#[export] Hint Constructors substitute_letrec : core.
-#[export] Hint Constructors substitute_binding : core.
+  Fixpoint substitute_bindings_nonrec (x : name) (s : Term) (bs : list Binding) : list Binding :=
+    match bs with
+    | nil => 
+        nil
+    | b :: bs' => 
+        if existsb (eqb x) (bound_vars_in_binding b)
+          then
+            substb x s b :: bs
+          else
+            substb x s b :: substitute_bindings_nonrec x s bs'
+    end.
 
-Scheme substitute__ind := Minimality for substitute Sort Prop
-  with substitute_letrec__ind := Minimality for substitute_letrec Sort Prop
-  with substitute_binding__ind := Minimality for substitute_binding Sort Prop.
+  Fixpoint substitute_bindings_rec (x : name) (s : Term) (bs : list Binding) : list Binding :=
+    match bs with
+    | nil =>
+        nil
+    | b :: bs' =>
+        substb x s b :: substitute_bindings_rec x s bs'
+    end.
 
-Combined Scheme substitute__mutind from 
-  substitute__ind, 
-  substitute_letrec__ind, 
-  substitute_binding__ind.
+End SubstBindings.
+
+Fixpoint substitute (x : name) (s : Term) (t : Term) {struct t} : Term :=
+  match t with
+  | Let NonRec bs t0 =>
+      Let NonRec (@substitute_bindings_nonrec substitute_binding x s bs)
+        (if existsb (eqb x) (bound_vars_in_bindings bs) 
+          then t0
+          else substitute x s t0
+        ) 
+  | Let Rec bs t0 =>
+      if existsb (eqb x) (bound_vars_in_bindings bs) 
+        then 
+          Let Rec bs t0
+        else
+          Let Rec (@substitute_bindings_rec substitute_binding x s bs) (substitute x s t0)
+  | Var y => 
+      if x =? y
+        then s
+        else Var y
+  | TyAbs bX K t0 =>
+      TyAbs bX K (substitute x s t0)
+  | LamAbs bx T t0 =>
+      if x =? bx
+        then LamAbs bx T t0
+        else LamAbs bx T (substitute x s t0)
+  | Apply t1 t2 =>
+      Apply (substitute x s t1) (substitute x s t2)
+  | Constant u =>
+      Constant u
+  | Builtin d =>
+      Builtin d
+  | TyInst t0 T =>
+      TyInst (substitute x s t0) T
+  | Error T =>
+      Error T
+  | IWrap F T t0 =>
+      IWrap F T (substitute x s t0)
+  | Unwrap t0 =>
+      Unwrap (substitute x s t0)
+  end
+
+with substitute_binding (x : name) (s : Term) (b : Binding) {struct b} : Binding :=
+  match b with
+  | TermBind stricty (VarDecl y T) tb =>
+      TermBind stricty (VarDecl y T) (substitute x s tb)
+  | _ => b
+  end.
+
+Notation "'[' s '/' x ']' t" := (substitute x s t) (in custom plutus_term at level 20, x constr).
+Notation "'[' s '/' x '][b]' b" := (substitute_binding x s b) (in custom plutus_term at level 20, x constr).
+Notation "'[' s '/' x '][bnr]' bs" := (@substitute_bindings_nonrec substitute_binding x s bs) (in custom plutus_term at level 20, x constr).
+Notation "'[' s '/' x '][br]' bs" := (@substitute_bindings_rec substitute_binding x s bs) (in custom plutus_term at level 20, x constr).
 
 (** * Multi-substitutions of types in type annotations *)
 
 Definition env := list (name * Term).
 
-Inductive msubst_term : env -> Term -> Term -> Prop :=
-  | msubst_term__nil : forall t,
-      msubst_term nil t t
-  | msubst_term__cons : forall x s ss t t' t'',
-      substitute x s t t' ->
-      msubst_term ss t' t'' ->
-      msubst_term ((x, s) :: ss) t t''
-  .
+Fixpoint msubst_term (ss : env) (t : Term) : Term :=
+  match ss with
+  | nil => t
+  | (x, s) :: ss' => msubst_term ss' <{ [s / x] t }>
+  end.
 
-Inductive msubst_binding : env -> Binding -> Binding -> Prop :=
-  | msubst_binding__nil : forall b,
-      msubst_binding nil b b
-  | msubst_binding__cons : forall x s ss b b' b'',
-      substitute_binding x s b b' ->
-      msubst_binding ss b' b'' ->
-      msubst_binding ((x, s) :: ss) b b''.
+Fixpoint msubst_binding (ss : env) (b : Binding) : Binding :=
+  match ss with
+  | nil => b
+  | (x, s) :: ss' => msubst_binding ss' <{ [s / x][b] b }>
+  end.
